store/client_proofs.v
@@ -1,0 +1,248 @@
+From stdpp Require Import base gmap.
+From mathcomp Require Import ssreflect.
+From stdpp Require Import namespaces.
+From iris.algebra Require Import agree auth csum gset gmap excl frac.
+From iris.algebra Require Import max_prefix_list.
+From iris.heap_lang Require Import notation proofmode.
+From cryptis Require Import lib version term cryptis primitives tactics.
+From cryptis Require Import role session pk_auth pk_dh.
+From cryptis.store Require Import impl shared.
+
+Set Implicit Arguments.
+Unset Strict Implicit.
+Unset Printing Implicit Defensive.
+
+Section Verif.
+
+Context `{!cryptisG Σ, !heapGS Σ, !sessionG Σ}.
+Notation iProp := (iProp Σ).
+
+Context `{!storeG Σ}.
+
+Local Instance STORE : PK := PK_DH (λ _ _ _ _, True)%I.
+
+Implicit Types (cs : cst) (ss : sst).
+Implicit Types kI kR kS t : term.
+Implicit Types n : nat.
+Implicit Types γ : gname.
+Implicit Types v : val.
+
+Variable N : namespace.
+
+Definition client_state kI kR s n t : iProp :=
+  cst_ts s ↦ #n ∗
+  sterm (cst_key s) ∗
+  version_auth (cst_name s) (DfracOwn 1) n t ∗
+  store_key N Init kI kR (cst_key s) (cst_ok s) (cst_name s).
+
+Lemma client_state_version_frag kI kR s n t :
+  client_state kI kR s n t -∗
+  version_frag (cst_name s) n t.
+Proof.
+iIntros "(_ & _ & ? & _)".
+by iApply version_auth_frag.
+Qed.
+
+Lemma client_state_store_key kI kR s n t :
+  client_state kI kR s n t -∗
+  sterm (cst_key s) ∗
+  store_key N Init kI kR (cst_key s) (cst_ok s) (cst_name s).
+Proof. by iIntros "(_ & ? & _ & ?)"; eauto. Qed.
+
+Lemma wp_client_get_ts E kI kR s n t :
+  {{{ client_state kI kR s n t }}}
+    Client.get_ts (repr s) @ E
+  {{{ RET #n; client_state kI kR s n t }}}.
+Proof.
+rewrite /Client.get_ts.
+iIntros "%Φ (Hl & #s_kS & Hγ & state) post".
+wp_pures. wp_load. iApply "post". iModIntro. by iFrame.
+Qed.
+
+Lemma wp_client_next_ts t' E kI kR s n t :
+  {{{ client_state kI kR s n t }}}
+    Client.next_ts (repr s) @ E
+  {{{ RET #(); client_state kI kR s (S n) t' }}}.
+Proof.
+iIntros "%Ψ (n_stored & #s_key & n_t & auth) post".
+iMod (version_update t' with "n_t") as "n_t".
+rewrite /Client.next_ts; wp_pures; wp_load; wp_store.
+iApply "post"; iFrame.
+rewrite (_ : (n + 1)%Z = (S n)%nat :> Z); last by lia.
+by iFrame.
+Qed.
+
+Lemma wp_client_get_sk E kI kR s n t :
+  {{{ client_state kI kR s n t }}}
+    Client.get_sk (repr s) @ E
+  {{{ RET (repr (Spec.mkskey (cst_key s))); client_state kI kR s n t }}}.
+Proof.
+rewrite /Client.get_sk.
+iIntros "%Φ ? post". wp_pures. by iApply "post".
+Qed.
+
+Lemma wp_client_send_store E kI kR c s n t t' :
+  ↑cryptisN ⊆ E →
+  channel c -∗
+  ctx N -∗
+  pterm t' -∗ (* FIXME: t' does not have to be public already *)
+  {{{ client_state kI kR s n t }}}
+    Client.send_store N c (repr s) t' @ E
+  {{{ RET #(); client_state kI kR s (S n) t' }}}.
+Proof.
+rewrite /Client.send_store.
+iIntros "% #chan_c (#? & _) #p_t' !> %Φ state post".
+wp_pures. wp_bind (Client.next_ts _).
+iApply (wp_client_next_ts t' with "state"); iIntros "!> state".
+iPoseProof (client_state_version_frag with "state") as "#frag".
+wp_pures. wp_bind (Client.get_ts _).
+iApply (wp_client_get_ts with "state"); iIntros "!> state".
+wp_pures. wp_bind (Client.get_sk _).
+iApply (wp_client_get_sk with "state"); iIntros "!> state".
+iPoseProof (client_state_store_key with "state") as "# (s_k & p_k)".
+wp_pures. wp_list. wp_bind (tint _). iApply wp_tint. wp_list.
+wp_term_of_list. wp_tsenc. wp_pures.
+iApply (wp_send with "[//]"); eauto; last by iApply "post".
+iModIntro. iApply pterm_TEncIS => //.
+- by rewrite sterm_TKey.
+- iModIntro. iExists (S n), t', kI, kR, (cst_ok s), (cst_name s).
+  by eauto.
+- rewrite sterm_of_list /= sterm_TInt; do ![iSplit => //].
+  by iApply pterm_sterm.
+- iModIntro. iIntros "_". rewrite pterm_of_list /= pterm_TInt. iSplit => //.
+  by iSplit => //.
+Qed.
+
+Lemma wp_client_ack_store E kI kR c s n t :
+  ↑cryptisN ⊆ E →
+  channel c -∗
+  ctx N -∗
+  {{{ client_state kI kR s n t }}}
+    Client.ack_store N c (repr s) @ E
+  {{{ RET #(); client_state kI kR s n t }}}.
+Proof.
+iIntros "% #chan_c (_ & #? & _) !> %Φ state post".
+rewrite /Client.ack_store. wp_pures.
+wp_bind (Client.get_ts _). iApply (wp_client_get_ts with "state") => //.
+iIntros "!> state". wp_pures.
+wp_bind (Client.get_sk _). iApply (wp_client_get_sk with "state") => //.
+iIntros "!> state". wp_pures.
+iPoseProof (client_state_store_key with "state") as "#[s_k ?]".
+iCombine "post state" as "I". iRevert "I".
+iApply wp_sess_recv => //. iIntros "!> %m [post state] _".
+wp_pures. wp_bind (tint _). iApply wp_tint.
+wp_eq_term e; wp_pures; iModIntro; last first.
+  iLeft. by iFrame.
+iRight. iExists _; iSplit => //. by iApply "post".
+Qed.
+
+Lemma wp_client_store E kI kR c s n t t' :
+  ↑cryptisN ⊆ E →
+  channel c -∗
+  ctx N -∗
+  pterm t' -∗
+  {{{ client_state kI kR s n t }}}
+    Client.store N c (repr s) t' @ E
+  {{{ RET #(); client_state kI kR s (S n) t' }}}.
+Proof.
+iIntros "% #chan_c #ctx #p_t' !> %Φ state post". rewrite /Client.store.
+wp_pures. wp_bind (Client.send_store _ _ _ _).
+iApply (wp_client_send_store with "[] [] [] [state] [post]") => //.
+iIntros "!> state". wp_pures.
+iApply (wp_client_ack_store with "[] [] [state] [post]") => //.
+Qed.
+
+Lemma wp_client_connect E c kI kR dq ph T :
+  ↑N ⊆ E →
+  ↑cryptisN ⊆ E →
+  channel c -∗
+  cryptis_ctx -∗
+  ctx N -∗
+  pterm (TKey Enc kI) -∗
+  pterm (TKey Enc kR) -∗
+  {{{ ●H{dq|ph} T }}}
+    Client.connect N c (TKey Dec kI) (TKey Enc kI) (TKey Enc kR) @ E
+  {{{ s, RET (repr s);
+      ●H{dq|ph} T ∗
+      ⌜cst_ok s = in_honest kI kR T⌝ ∗
+      client_state kI kR s 0 (TInt 0) }}}.
+Proof.
+iIntros "% % #chan_c #ctx (_ & _ & _ & _ & #ctx' & #key) #p_ekI #p_ekR".
+iIntros "!> %Φ hon post". rewrite /Client.connect. wp_pures.
+iCombine "hon post" as "post". iRevert "post".
+iApply wp_do_until. iIntros "!> [hon post]". wp_pures.
+wp_bind (pk_dh_init _ _ _ _ _).
+iApply (wp_pk_dh_init with "[] [] [] [] [] [hon]"); eauto.
+  by iFrame.
+iIntros "!> %okS [hon HokS]".
+case: okS => [kS|]; wp_pures; last by iLeft; iFrame; eauto.
+wp_alloc l as "Hl". wp_pures. wp_tag. wp_bind (mkskey _). iApply wp_mkskey.
+iMod version_alloc as "[%γ cur_term]".
+wp_pures. iRight. iExists _. iSplitR; eauto.
+iDestruct "HokS" as "(#s_kS & _ & #sessW & status)".
+iApply ("post" $! {| cst_ts := l; cst_key := Spec.tag (N.@"key") kS;
+                     cst_name := γ;
+                     cst_ok := in_honest kI kR T |}).
+rewrite /client_state /=. iFrame. rewrite sterm_tag.
+do 2!iSplitR => //.
+iExists kS, ph, T. do 3!iSplitR => //.
+case: in_honest; last by eauto.
+iDestruct "status" as "(#p_kS & token & #session)".
+iMod (term_meta_set _ _ γ N with "token") as "#meta"; eauto.
+iModIntro. do 2!iSplit => //. iIntros "!> %kt #p_kS'".
+rewrite (pterm_TKey kt) pterm_tag sterm_tag.
+iDestruct "p_kS'" as "[?|[_ p_kS']]"; first by iApply "p_kS".
+by iMod (wf_key_elim with "p_kS' key") as "#[]".
+Qed.
+
+Lemma wp_client_load E c kI kR s n t :
+  ↑N ⊆ E →
+  ↑cryptisN ⊆ E →
+  channel c -∗
+  ctx N -∗
+  pterm (TKey Enc kI) -∗
+  pterm (TKey Enc kR) -∗
+  {{{ client_state kI kR s n t }}}
+    Client.load N c (repr s) @ E
+  {{{ t', RET (repr t');
+      client_state kI kR s n t ∗
+      ◇ ⌜cst_ok s → t' = t⌝ }}}.
+Proof.
+iIntros "% % #chan_c #ctx #p_ekI #p_ekR !> %Φ state post".
+iDestruct "ctx" as "(_ & _ & ? & ? & _)".
+rewrite /Client.load. wp_pures.
+wp_bind (Client.get_ts _). iApply (wp_client_get_ts with "state").
+iIntros "!> state". wp_pures. wp_bind (tint _). iApply wp_tint.
+wp_pures. wp_bind (Client.get_sk _).
+iApply (wp_client_get_sk with "state"). iIntros "!> state". wp_pures.
+wp_tsenc. wp_pures.
+iPoseProof (client_state_store_key with "state") as "#[s_k status]".
+wp_bind (send _ _). iApply wp_send; eauto.
+  iModIntro. iApply pterm_TEncIS; eauto.
+  - by rewrite sterm_TKey.
+  - by rewrite sterm_TInt.
+  - rewrite pterm_TInt. by eauto.
+wp_pures.
+iCombine "post state" as "I". iRevert "I". iApply wp_sess_recv => //.
+iIntros "!> %ts [post state] #p_t'". wp_pures.
+wp_list_of_term ts; wp_pures; last by iLeft; iFrame.
+wp_list_match => [n' v -> {ts}|_]; wp_pures; last by iLeft; iFrame.
+wp_eq_term e; wp_pures; last by iLeft; iFrame.
+subst n'. iModIntro. iRight. iExists _; iSplit; eauto.
+iApply ("post" $! v). iSplit => //.
+case e_ok: (cst_ok s) => //=. iIntros "_".
+iPoseProof "status"
+  as "(%kS' & %ph & %T & %e_kS & #hon & #sess & #meta & #? & #p_kS)".
+iDestruct "p_t'" as "[[contra _] | succ]".
+  iMod ("p_kS" $! Enc with "contra") as "{contra} #[]".
+iDestruct "succ" as "(_ & #wf_t' & _)".
+iDestruct "wf_t'" as "(%n' & %t' & %e & tP)".
+iDestruct "state" as "(_ & _ & auth & _)".
+case/Spec.of_list_inj: e => /Nat2Z.inj <- <- {n' t'}.
+iModIntro.
+iApply "tP".
+- by iApply "status".
+- by iApply version_auth_frag.
+Qed.
+
+End Verif.
