store/impl.v
@@ -1,0 +1,160 @@
+From stdpp Require Import base gmap.
+From mathcomp Require Import ssreflect.
+From stdpp Require Import namespaces.
+From iris.algebra Require Import agree auth csum gset gmap excl frac.
+From iris.algebra Require Import max_prefix_list.
+From iris.heap_lang Require Import notation proofmode.
+From cryptis Require Import lib version term cryptis primitives tactics.
+From cryptis Require Import role session pk_auth pk_dh.
+
+Set Implicit Arguments.
+Unset Strict Implicit.
+Unset Printing Implicit Defensive.
+
+Record cst := {
+  cst_ts   : loc;
+  cst_key  : term;
+  cst_name : gname;
+  cst_ok   : bool;
+}.
+
+#[global]
+Instance cst_repr : Repr cst := λ s, (#(cst_ts s), Spec.mkskey (cst_key s))%V.
+
+(* FIXME: Maybe generalize this *)
+Definition sess_recv N : val := λ: "c" "k" "f",
+  do_until (λ: <>,
+    let: "m" := recv "c" in
+    bind: "m" := tsdec N "k" "m" in
+    "f" "m"
+  ).
+
+Module Client.
+
+Section Client.
+
+Variable N : namespace.
+
+Definition connect : val := λ: "c" "skA" "pkA" "pkB",
+  do_until (λ: <>,
+    bind: "kS" := pk_dh_init N "c" "skA" "pkA" "pkB" in
+    let: "l"  := ref #0 in
+    let: "kS" := mkskey (tag (N.@"key") "kS") in
+    SOME ("l", "kS")
+  ).
+
+Definition get_ts : val := λ: "cs",
+  let: "l" := Fst "cs" in
+  !"l".
+
+Definition next_ts : val := λ: "cs",
+  let: "l" := Fst "cs" in
+  "l" <- (!"l" + #1).
+
+Definition get_sk : val := λ: "cs",
+  Snd "cs".
+
+Definition send_store : val := λ: "c" "cs" "v",
+  next_ts "cs";;
+  let: "n" := get_ts "cs" in
+  let: "sk" := get_sk "cs" in
+  let: "m" := tsenc (N.@"store") "sk" (term_of_list [tint "n"; "v"]) in
+  send "c" "m".
+
+Definition ack_store : val := λ: "c" "cs",
+  let: "n" := get_ts "cs" in
+  let: "sk" := get_sk "cs" in
+  sess_recv (N.@"ack_store") "c" "sk" (λ: "m",
+    assert: eq_term "m" (tint "n") in
+    SOME #()
+  ).
+
+Definition store : val := λ: "c" "cs" "t",
+  send_store "c" "cs" "t";;
+  ack_store "c" "cs".
+
+Definition load : val := λ: "c" "cs",
+  let: "n" := tint (get_ts "cs") in
+  let: "sk" := get_sk "cs" in
+  send "c" (tsenc (N.@"load") "sk" "n");;
+  sess_recv (N.@"ack_load") "c" "sk" (λ: "resp",
+    bind: "resp" := list_of_term "resp" in
+    list_match: ["n'"; "t"] := "resp" in
+    assert: eq_term "n'" "n" in
+    SOME "t"
+  ).
+
+End Client.
+
+End Client.
+
+Record sst := {
+  sst_ts   : loc;
+  sst_val  : loc;
+  sst_key  : term;
+  sst_name : gname;
+  sst_ok   : bool;
+}.
+
+#[global]
+Instance sst_repr : Repr sst :=
+  λ ss, (#(sst_ts ss), #(sst_val ss), Spec.mkskey (sst_key ss))%V.
+
+Module Server.
+
+Implicit Types N : namespace.
+
+Definition get_ts : val := λ: "ss",
+  !(Fst (Fst "ss")).
+
+Definition get_val : val := λ: "ss",
+  !(Snd (Fst "ss")).
+
+Definition upd_val : val := λ: "ss" "ts" "v",
+  Fst (Fst "ss") <- "ts" ;;
+  Snd (Fst "ss") <- "v".
+
+Definition get_key : val := λ: "ss",
+  Snd "ss".
+
+Definition handle_store N : val := λ: "c" "ss" "m",
+  bind: "m" := list_of_term "m" in
+  list_match: ["n"; "x"] := "m" in
+  bind: "n'" := to_int "n" in
+  assert: get_ts "ss" ≤ "n'" in
+  upd_val "ss" "n'" "x";;
+  send "c" (tsenc (N.@"ack_store") (get_key "ss") "n").
+
+Definition handle_load N : val := λ: "c" "ss" "m",
+  bind: "n" := to_int "m" in
+  assert: get_ts "ss" = "n" in
+  let: "v" := get_val "ss" in
+  send "c" (tsenc (N.@"ack_load") (get_key "ss") (term_of_list ["m"; "v"])).
+
+Definition conn_handler_body N : val := λ: "c" "ss",
+  let: "sk" := get_key "ss" in
+  let: "m" := recv "c" in
+  match: tsdec (N.@"store") "sk" "m" with
+    SOME "m" => handle_store N "c" "ss" "m"
+  | NONE => match: tsdec (N.@"load") "sk" "m" with
+    SOME "m" => handle_load N "c" "ss" "m"
+  | NONE => #()
+  end end.
+
+Definition conn_handler N : val := rec: "loop" "c" "ss" :=
+  conn_handler_body N "c" "ss";;
+  "loop" "c" "ss".
+
+Definition listen N : val := rec: "loop" "c" "skB" "pkB" :=
+  match: pk_dh_resp N "c" "skB" "pkB" with
+    NONE =>
+    "loop" "c" "skB" "pkB"
+  | SOME "res" =>
+    let: "pkA" := Fst "res" in
+    let: "kS"  := mkskey (tag (N.@"key") (Snd "res")) in
+    let: "ss"  := (ref #0, ref #0, "ks") in
+    Fork (conn_handler N "c" "ss");;
+    "loop" "c" "skB" "pkB"
+  end.
+
+End Server.
