store/server_proofs.v
@@ -1,0 +1,176 @@
+From stdpp Require Import base gmap.
+From mathcomp Require Import ssreflect.
+From stdpp Require Import namespaces.
+From iris.algebra Require Import agree auth csum gset gmap excl frac.
+From iris.algebra Require Import max_prefix_list.
+From iris.heap_lang Require Import notation proofmode.
+From cryptis Require Import lib version term cryptis primitives tactics.
+From cryptis Require Import role session pk_auth pk_dh.
+From cryptis.store Require Import impl shared.
+
+Set Implicit Arguments.
+Unset Strict Implicit.
+Unset Printing Implicit Defensive.
+
+Section Verif.
+
+Context `{!cryptisG Σ, !heapGS Σ, !sessionG Σ}.
+Notation iProp := (iProp Σ).
+
+Context `{!storeG Σ}.
+
+Local Instance STORE : PK := PK_DH (λ _ _ _ _, True)%I.
+
+Implicit Types (cs : cst) (ss : sst).
+Implicit Types kI kR kS t : term.
+Implicit Types n : nat.
+Implicit Types γ : gname.
+Implicit Types v : val.
+
+Variable N : namespace.
+
+Definition server_state kI kR s n t : iProp :=
+  sst_ts s ↦ #n ∗
+  sst_val s ↦ repr t ∗
+  sterm (sst_key s) ∗
+  pterm t ∗
+  (if sst_ok s then version_frag (sst_name s) n t else True%I) ∗
+  store_key N Resp kI kR (sst_key s) (sst_ok s) (sst_name s).
+
+Lemma wp_server_get_ts E kI kR ss n t :
+  {{{ server_state kI kR ss n t }}}
+    Server.get_ts (repr ss) @ E
+  {{{ RET #n; server_state kI kR ss n t }}}.
+Proof.
+iIntros "%Φ (ts & val & ?) post".
+rewrite /Server.get_ts. wp_pures. wp_load. iApply "post".
+by iFrame.
+Qed.
+
+Lemma wp_server_upd_val E kI kR ss n t n' t' :
+  {{{ ▷ server_state kI kR ss n t ∗
+      ▷ pterm t' ∗
+      ▷ if sst_ok ss then version_frag (sst_name ss) n' t' else True%I }}}
+    Server.upd_val (repr ss) #n' t' @ E
+  {{{ RET #(); server_state kI kR ss n' t' }}}.
+Proof.
+iIntros "%Φ ((ts & val & ? & ? & #frag & key) & p_t' & #frag') post".
+rewrite /Server.upd_val. wp_pures. wp_store. wp_pures. wp_store.
+iApply "post". iFrame.
+by case: sst_ok.
+Qed.
+
+Lemma wp_server_get_val E kI kR ss n t :
+  {{{ server_state kI kR ss n t }}}
+    Server.get_val (repr ss) @ E
+  {{{ RET (repr t);
+      pterm t ∗
+      (if sst_ok ss then version_frag (sst_name ss) n t else True%I) ∗
+      server_state kI kR ss n t }}}.
+Proof.
+iIntros "%Φ (ts & val & ? & #? & #frag & ?) post".
+rewrite /Server.get_val. wp_pures. wp_load. iApply "post".
+iFrame.
+by eauto.
+Qed.
+
+Lemma wp_server_get_key E kI kR ss n t :
+  {{{ server_state kI kR ss n t }}}
+    Server.get_key (repr ss) @ E
+  {{{ RET (repr (Spec.mkskey (sst_key ss)));
+      server_state kI kR ss n t }}}.
+Proof.
+iIntros "%Φ ? post".
+rewrite /Server.get_key. wp_pures. by iApply "post".
+Qed.
+
+Lemma store_predE kI kR ss n t (n' : nat) t' :
+  server_state kI kR ss n t -∗
+  ctx N -∗
+  pterm (TEnc (sst_key ss) (Spec.tag (N.@"store") (Spec.of_list [TInt n'; t']))) -∗
+  ▷ (server_state kI kR ss n t ∗
+     pterm t' ∗
+     if sst_ok ss then version_frag (sst_name ss) n' t' else True%I).
+Proof.
+iIntros "state #(? & ? & _ & _) #p_m".
+iPoseProof (pterm_TEncE with "p_m [//]") as "{p_m} p_m".
+iDestruct "state" as "(? & ? & #? & #p_t & #frag & key)".
+iDestruct "key" as "(%kS & %ph & %T & %e_key & %e_ok & #sessW & #key)".
+rewrite pterm_of_list /=.
+iDestruct "p_m" as "[(p_key & _ & p_t' & _) | p_m]".
+{ case e: sst_ok; last first.
+    do 2?iSplit => //.
+    iFrame. rewrite e. do 3!iSplit => //.
+    iExists kS, _, T; iSplit => //.
+    rewrite -e_ok e; iSplit => //.
+    by iSplit => //.
+  iDestruct "key" as "(#meta & #key & #contra)".
+  iDestruct ("contra" with "p_key") as ">[]". }
+iDestruct "p_m" as "(#p_m & s_t' & _)".
+iDestruct "p_m" as "(%n'' & %t'' & %kI'' & %kR'' & %ok'' & %γ'' & >%e & p_m)".
+case/Spec.of_list_inj: e => /Nat2Z.inj <- <- {n'' t''}.
+iDestruct "p_m" as "(p_t' & >frag'' & p_m)".
+case e: sst_ok; last first.
+  iModIntro. do 2?iSplit => //.
+  iFrame. iSplit => //. iSplit => //. rewrite e. iSplit => //.
+  iExists kS, ph, T; iSplit => //.
+  rewrite -e_ok e; iSplit => //.
+  by iSplit => //.
+iDestruct "key" as "(#meta & #key & #s_key)".
+iModIntro.
+iDestruct "p_m" as "(%kS''' & %ph''' & %T''' & %e_key''' & p_m)".
+have {kS''' e_key'''} -> : kS''' = kS.
+  rewrite e_key''' in e_key.
+  by have [??] := Spec.tag_inj _ _ _ _ e_key.
+iDestruct "p_m" as "(%e_ok''' & sessW''' & sess''')".
+iDestruct (session_weak_session_key with "sessW''' key")
+  as "(-> & -> & -> & ->)".
+rewrite e_ok''' -e_ok e.
+iDestruct "sess'''" as "(meta''' & _)".
+iPoseProof (term_meta_agree with "meta''' meta") as "->".
+iFrame. rewrite e.
+do 4?iSplit => //.
+iExists kS, ph, T. rewrite -e_ok e. do 5?iSplit => //.
+Qed.
+
+Lemma ack_storeI kS n :
+  ctx N -∗
+  sterm kS -∗
+  pterm (TEnc kS (Spec.tag (N.@"ack_store") (TInt n))).
+Proof.
+iIntros "(_ & #ctx & _) #s_kS".
+iApply pterm_TEncIS => //.
+- by rewrite sterm_TKey.
+- iModIntro. by iExists n.
+- by rewrite sterm_TInt.
+- by rewrite pterm_TInt; eauto.
+Qed.
+
+Lemma wp_server_handle_store E c kI kR ss n t m :
+  ↑cryptisN ⊆ E →
+  channel c -∗
+  ctx N -∗
+  pterm (TEnc (sst_key ss) (Spec.tag (N.@"store") m)) -∗
+  {{{ server_state kI kR ss n t }}}
+    Server.handle_store N c (repr ss) m @ E
+  {{{ n' t' v, RET v; server_state kI kR ss n' t' }}}.
+Proof.
+iIntros "%sub #chan_c #ctx #p_m !> %Φ state post".
+rewrite /Server.handle_store. wp_pures.
+wp_list_of_term m; wp_pures; last by iApply "post".
+wp_list_match => [n' t' ->|_]; wp_pures; last by iApply "post".
+wp_bind (to_int _). iApply wp_to_int.
+case: Spec.to_intP => [ {}n' -> | _]; wp_pures; last by iApply "post".
+wp_bind (Server.get_ts _). iApply (wp_server_get_ts with "state").
+iIntros "!> state". wp_pures.
+case: bool_decide_reflect => [nn'|_]; wp_pures; last by iApply "post".
+have {n' nn'} [n' ->] : ∃ n'' : nat, n' = n''.
+  exists (Z.to_nat n'). by lia.
+iPoseProof (store_predE with "state ctx p_m") as "(state & #p_t' & #frag)".
+wp_bind (Server.upd_val _ _ _).
+iApply (wp_server_upd_val with "[$]").
+iIntros "!> state". wp_pures.
+wp_bind (Server.get_key _). iApply wp_server_get_key => //.
+Admitted.
+
+End Verif.
