store/shared.v
@@ -1,0 +1,106 @@
+From stdpp Require Import base gmap.
+From mathcomp Require Import ssreflect.
+From stdpp Require Import namespaces.
+From iris.algebra Require Import agree auth csum gset gmap excl frac.
+From iris.algebra Require Import max_prefix_list.
+From iris.heap_lang Require Import notation proofmode.
+From cryptis Require Import lib version term cryptis primitives tactics.
+From cryptis Require Import role session pk_auth pk_dh.
+From cryptis.store Require Import impl.
+
+Set Implicit Arguments.
+Unset Strict Implicit.
+Unset Printing Implicit Defensive.
+
+Section Defs.
+
+Context `{!cryptisG Σ, !heapGS Σ, !sessionG Σ}.
+Notation iProp := (iProp Σ).
+
+Class storeG := StoreG {
+  store_inG :> inG Σ (authR (max_prefix_listUR termO));
+}.
+
+Context `{!storeG}.
+
+Local Instance STORE : PK := PK_DH (λ _ _ _ _, True)%I.
+
+Implicit Types (cs : cst) (ss : sst).
+Implicit Types kI kR kS t : term.
+Implicit Types n : nat.
+Implicit Types γ : gname.
+Implicit Types v : val.
+
+(* FIXME: infer the invariant φ in a tactic, similarly to how iLöb works *)
+Lemma wp_sess_recv E N c sk (f : val) φ Φ Ψ :
+  ↑cryptisN ⊆ E →
+  channel c -∗
+  enc_pred N Φ -∗
+  sterm sk -∗
+  □ (∀ t,
+      φ -∗
+      ▷ (pterm (TKey Enc sk) ∗ pterm t ∨
+         sterm t ∗ □ Φ sk t ∗ □ (pterm (TKey Dec sk) → pterm t)) -∗
+      WP f t @ E {{ v, ⌜v = NONEV⌝ ∗ φ ∨ ∃ v', ⌜v = SOMEV v'⌝ ∗ Ψ v' }}) -∗
+  φ -∗ WP sess_recv N c (Spec.mkskey sk) f @ E {{ Ψ }}.
+Proof.
+iIntros "% #chan_c #ΦP #s_sk #wp_f Hφ"; rewrite /sess_recv; wp_pures.
+iRevert "Hφ". iApply wp_do_until; iIntros "!> Hφ". wp_pures.
+wp_bind (recv _); iApply wp_recv => //.
+iIntros "%t #p_t"; wp_pures.
+wp_tsdec_eq t' e; wp_pures; eauto.
+rewrite {}e {t} pterm_TEnc.
+iApply ("wp_f" with "Hφ"). rewrite pterm_tag.
+iDestruct "p_t" as "[[??] | p_t]"; eauto.
+iRight. rewrite sterm_TEnc sterm_tag.
+iDestruct "p_t" as "[[??] [inv_t' p_t]]".
+do 2![iSplit => //].
+iPoseProof (wf_enc_elim with "inv_t' ΦP") as "{inv_t'} #inv_t'".
+eauto.
+Qed.
+
+Variable N : namespace.
+
+Definition store_key rl kI kR kS ok γ : iProp := ∃ kS' ph T,
+  ⌜kS = Spec.tag (N.@"key") kS'⌝ ∗
+  ⌜ok = in_honest kI kR T⌝ ∗
+  pk_dh_session_weak N (λ _ _ _ _, True)%I rl kI kR kS' ph T ∗
+  if ok then
+    pk_dh_session_meta N (λ _ _ _ _, True)%I Init kI kR kS' N γ ∗
+    pk_dh_session_key N (λ _ _ _ _, True)%I kI kR kS' ph T ∗
+    □ (∀ kt, pterm (TKey kt kS) -∗ ◇ False)
+  else True%I.
+
+#[global]
+Instance store_key_persistent rl kI kR kS ok γ :
+  Persistent (store_key rl kI kR kS ok γ).
+Proof. apply _. Qed.
+
+Definition store_pred kS m : iProp := ∃ (n : nat) t kI kR ok γ,
+  ⌜m = Spec.of_list [TInt n; t]⌝ ∗
+  pterm t ∗
+  version_frag γ n t ∗
+  store_key Init kI kR kS ok γ.
+
+Definition ack_store_pred kS m : iProp := ∃ (n : nat),
+  ⌜m = TInt n⌝. (* FIXME: Do we need anything else here? *)
+
+Definition load_pred (kS m : term) : iProp := True.
+
+Definition ack_load_pred kS m : iProp := ∃ (n : nat) t,
+  ⌜m = Spec.of_list [TInt n; t]⌝ ∗
+  ∀ kI kR γ t', store_key Init kI kR kS true γ -∗
+  version_frag γ n t' -∗
+  ⌜t = t'⌝.
+
+Definition ctx : iProp :=
+  enc_pred (N.@"store") store_pred ∗
+  enc_pred (N.@"ack_store") ack_store_pred ∗
+  enc_pred (N.@"load") load_pred ∗
+  enc_pred (N.@"ack_load") ack_load_pred ∗
+  pk_dh_ctx N (λ _ _ _ _, True)%I ∗
+  key_pred (N.@"key") (λ _ _, False)%I.
+
+End Defs.
+
+Arguments storeG Σ : clear implicits.
